MECMAR/props/Definitions.v
@@ -1,0 +1,13 @@
+From Coq Require Import ZArith.
+From Warblre Require Import Tactics Specialize Focus Result Base Patterns StaticSemantics Notation Semantics.
+Import Result.Notations.
+
+(* Notation for MatchStates which goes nicely with the normalization tactic *)
+Notation "s '[@' n '$' c ']'" := (match_state s n c) (at level 50, left associativity).
+
+(* Notation for the "tiny step" done in a character class matcher *)
+Notation "'step{' dir '}' e " := (if Direction.eqb dir forward then (e + 1)%Z else (e - 1)%Z) (at level 51, right associativity).
+
+Module Definitions.
+  Definition characterClass_successful_state input endIndex captures (dir: direction) := input [@ step{dir} endIndex $ captures ].
+End Definitions.
